Checkpoint while figuring out PDTM approach

Tealeaves/Adapters/PolyToMono/Kleisli/DecoratedTraversableFunctor.v
@@ -16,6 +16,8 @@ Import DecoratedTraversableCommIdemFunctor.Notations.
 
 #[local] Generalizable Variables ϕ T W G A B C D F M.
 
+(** * Parameterized Decorated Traversable Functor to single DTF *)
+(**********************************************************************)
 Section dtfp_to_dtf.
 
   Context
@@ -57,7 +59,8 @@ Section dtfp_to_dtf.
 
 End dtfp_to_dtf.
 
-
+(** * Parameterized Decorated Traversable Functor to single DTF *)
+(**********************************************************************)
 Section dtfp_to_dtf_bin.
 
   Context
@@ -145,3 +148,192 @@ Section relating.
 
 End relating.
 
+
+(** * Derived Monomorphic Instances *)
+(**********************************************************************)
+
+(** ** Derived Monomorphic Operations *)
+(**********************************************************************)
+Module DerivedOperations.
+  Section decorated_traversable_functor_derived_operations.
+
+    Context
+      `{DecoratedTraversableFunctorPoly T}.
+
+    Context {B: Type}.
+
+    #[export] Instance Mapdt_Mapdtp: Mapdt (list B) (T B) :=
+      fun G MapG PureG MultG A1 A2 f =>
+        mapdtp (T := T) (G := G)
+          (pure (F := G) ∘ extract) f.
+
+    (*
+    #[export] Instance Traversep_Mapdtp: Traverse2 T :=
+      fun A1 A2 B1 B2 G MapG PureG MultG g f =>
+        mapdtp (T := T) (G := G)
+          (g ∘ extract) (f ∘ extract).
+     *)
+
+  End decorated_traversable_functor_derived_operations.
+End DerivedOperations.
+
+(*
+(** ** Derived Typeclass Instances *)
+(**********************************************************************)
+Module DerivedInstances.
+  Section decorated_traversable_functor_derived_instances.
+
+    Import DerivedOperations.
+
+    Context
+      `{DecoratedTraversableFunctorPoly T}.
+
+    Context {B: Type}.
+
+    #[export] Instance DecoratedTraversableFunctor_DTFP:
+      DecoratedTraversableFunctor (list B) (T B).
+    Proof.
+      constructor.
+      - intro A.
+        unfold_ops @Mapdt_Mapdtp.
+        unfold_ops @Pure_I.
+        change (id ∘ ?x) with x.
+        rewrite kdtfp_mapdtp1.
+        reflexivity.
+      - intros.
+        unfold_ops @Mapdt_Mapdtp.
+        rewrite kdtfp_mapdtp2.
+        2:{
+          typeclasses eauto.
+        }
+        fequal.
+        { unfold kc3_ci.
+          ext [w b].
+          unfold compose.
+          unfold mapdt_ci.
+          unfold Mapdt_CommIdem_Z.
+          cbn.
+          rewrite map_ap.
+          rewrite map_ap.
+          rewrite app_pure_natural.
+          change (pure (F := G1) ○ extract)
+            with (pure (F := G1) ∘ extract (W := prod (list B)) (A := B)).
+          rewrite <- traverse_map.
+          rewrite (traverse_purity1 (T := list)).
+          unfold compose.
+          rewrite ap2.
+          rewrite ap2.
+          reflexivity.
+        }
+        { unfold kc_dtfp, kc3.
+          ext [ctx a].
+          unfold mapdt_ci.
+          unfold Mapdt_CommIdem_list_prefix.
+          rewrite map_ap.
+          rewrite map_ap.
+          rewrite app_pure_natural.
+          unfold mapdt_list_prefix.
+          unfold compose at 4.
+          rewrite <- traverse_map.
+          rewrite (traverse_purity1 (T := list)).
+          unfold compose at 4.
+          rewrite ap2.
+          rewrite <- map_to_ap.
+          unfold compose.
+          cbn.
+          compose near (f (ctx, a)) on right.
+          rewrite (fun_map_map (F := G1)).
+          fequal.
+          ext b.
+          unfold compose.
+          compose near ctx.
+          rewrite decorate_prefix_list_extract.
+          reflexivity.
+        }
+      - intros.
+        unfold_ops @Mapdt_Mapdtp.
+        rewrite kdtfp_morphism.
+        reassociate <- on left.
+        rewrite appmor_pure_pf.
+        reflexivity.
+    Qed.
+
+  End decorated_traversable_functor_derived_instances.
+
+  Export Kleisli.DecoratedTraversableFunctor.DerivedOperations.
+  Export Kleisli.DecoratedTraversableFunctor.DerivedInstances.
+
+End DerivedInstances.
+
+(*
+(** ** Relating Polymorphic and Monomorphic Operations *)
+(**********************************************************************)
+Section decorated_traversable_functor_polymorphic_monomorphic.
+
+  Import DerivedOperations.
+  Import DerivedInstances.
+
+  Context
+    `{DecoratedTraversableFunctorPoly T}.
+
+  Section monomorphic_binders.
+
+    Definition rename_variables {B A1 A2}:
+      (list B * A1 -> A2) -> T B A1 -> T B A2 :=
+      fun f => mapd (T := T B) f.
+
+    Definition rename_binders {A B1 B2}:
+      (list B1 * B1 -> B2) -> T B1 A -> T B2 A :=
+      fun f => mapdtp (G := fun A => A) f (extract).
+
+    Context {A1 A2 B1 B2}
+      (g: list B1 * B1 -> B2)
+      (f: list B2 * A1 -> A2).
+
+    Lemma rename_binders_variables_commute:
+      rename_variables f ∘ rename_binders g =
+        rename_binders g ∘ rename_variables
+          (fun '(ctx, a) =>
+             f (mapdt_ci (W := Z) (G := fun A => A) g ctx, a)).
+    Proof.
+      unfold rename_variables, rename_binders.
+      unfold_ops @Mapd_Mapdt.
+      unfold_ops @Mapdt_Mapdtp.
+
+      change (mapdtp (T := T) (G := fun A => A) ?g f) with
+        (map (F := fun A => A) (mapdtp (T := T) g f)).
+      rewrite (kdtfp_mapdtp2 (G1 := fun A => A) (G2 := fun A => A)).
+      2:{ intros [ctx b].
+          constructor; constructor; reflexivity. }
+      change (mapdtp (T := T) (G := fun A => A)
+                g ?ext)
+        with
+        (map (F := fun A => A)
+           (mapdtp (T := T) (G := fun A => A)
+              g ext)).
+      rewrite (kdtfp_mapdtp2 (G1 := fun A => A) (G2 := fun A => A)).
+      2:{ intros [ctx b].
+          constructor; constructor; reflexivity. }
+      fequal.
+      {
+        unfold kc3_ci.
+        ext [w b].
+        unfold_ops @Map_I.
+        unfold_ops @Mapdt_CommIdem_Z.
+        repeat reassociate <-.
+        rewrite <- (traverse_map (G2 := fun A => A) (T := Z)).
+        rewrite traverse_purity1.
+        rewrite <- map_to_traverse.
+        unfold_ops @Pure_I.
+        unfold compose, id; cbn.
+        unfold id.
+        compose near w.
+        rewrite decorate_prefix_list_extract.
+        reflexivity.
+      }
+    Qed.
+
+  End monomorphic_binders.
+End decorated_traversable_functor_polymorphic_monomorphic.
+*)
+*)
