Tealeaves/Classes/Categorical/DecoratedTraversableFunctorPoly.v
@@ -1,12 +1,20 @@
 From Tealeaves Require Export
   Classes.Categorical.DecoratedFunctorPoly
   Classes.Categorical.TraversableFunctor2
+  Classes.Categorical.DecoratedTraversableFunctor
   Classes.Categorical.ApplicativeCommutativeIdempotent
   Classes.Categorical.Monad
   Functors.List
   Functors.Writer.
 
 #[local] Generalizable Variables T F G W A B C.
+
+From Tealeaves Require Import
+  Adapters.PolyToMono.Categorical.DecoratedFunctor
+  Adapters.PolyToMono.Categorical.TraversableFunctor.
+
+Import PolyToMono.Categorical.DecoratedFunctor.ToMono1.
+Import PolyToMono.Categorical.TraversableFunctor.ToMono.
 
 (** * Polymorphic Decorated Traversable Functor *)
 (**********************************************************************)
@@ -17,6 +25,7 @@ Class DecoratedTraversableFunctorPoly
     dtfp_functor :> Functor2 T;
     dtfp_decorated :> DecoratedFunctorPoly T;
     dtfp_traversable :> TraversableFunctor2 T;
+    dtfp_vdist_dec :> forall (B: Type), DecoratedTraversableFunctor (list B) (T B);
     dtfp_dist2_decpoly:
     forall (B V: Type) `{ApplicativeCommutativeIdempotent G},
       dist2 (G := G) ∘ map2 (dist Z G) (dist2 (T := L)) ∘ (decp (B := G B) (V := G V)) =
