Tealeaves/Adapters/MonoidHom/Categorical.v
@@ -1,0 +1,102 @@
+From Tealeaves Require Export
+  Classes.Categorical.DecoratedFunctor
+  Classes.Categorical.DecoratedMonad
+  Classes.Categorical.DecoratedTraversableFunctor
+  Classes.Categorical.DecoratedTraversableMonad
+  Classes.Monoid
+  Functors.Writer.
+
+Import Applicative.Notations.
+Import Monoid.Notations.
+Import Product.Notations.
+
+#[local] Generalizable Variables ϕ T W G A B C D F M.
+
+Section dtm_to_dtm.
+
+  Context
+    {T: Type -> Type}
+    `{Dec_orig: Decorate W1 T}
+    `{Monoid W1}
+    `{Monoid W2}
+    (ϕ: W1 -> W2)
+    `{! Monoid_Morphism W1 W2 ϕ}.
+
+  Context
+    `{Map_T: Map T}
+    `{Dist_T: ApplicativeDist T}
+    `{Join_T: Join T}
+    `{Return_T: Return T}.
+
+  #[export] Instance Decorate_Monoid_Morphism: Decorate W2 T :=
+    fun A t => map (F := T) (map_fst ϕ) (dec T t).
+
+  #[export] Instance Natural_Decorate_Monoid_Morphism `{! DecoratedFunctor W1 T}:
+    Natural (@dec W2 T Decorate_Monoid_Morphism).
+  Proof.
+    constructor.
+    - typeclasses eauto.
+    - typeclasses eauto.
+    - intros. unfold_ops @Decorate_Monoid_Morphism.
+      unfold_ops @Map_compose.
+      ext t.
+      unfold compose at 1.
+      compose near (dec (Decorate := Dec_orig) T (A := A) t).
+      rewrite (fun_map_map (F := T)).
+      unfold compose at 2.
+      compose near t on right.
+      rewrite <- (natural (ϕ := @dec W1 T _)).
+      unfold compose at 2.
+      compose near (dec (Decorate := Dec_orig) T (A := A) t) on right.
+      unfold_ops @Map_compose.
+      rewrite (fun_map_map (F := T)).
+      rewrite product_map_commute.
+      reflexivity.
+  Qed.
+
+  #[export] Instance DecoratedFunctor_Monoid_Morphism `{! DecoratedFunctor W1 T}:
+    DecoratedFunctor W2 T.
+  Proof.
+    constructor.
+    - typeclasses eauto.
+    - typeclasses eauto.
+    - admit.
+    - admit.
+  Admitted.
+
+
+  #[export] Instance DecoratedMonad_Monoid_Morphism `{! DecoratedMonad W1 T}:
+    DecoratedMonad W2 T.
+  Proof.
+    constructor.
+    - typeclasses eauto.
+    - typeclasses eauto.
+    - typeclasses eauto.
+    - intros. unfold compose. admit.
+    - admit.
+  Admitted.
+
+
+  #[export] Instance DecoratedTraversableFunctor_Monoid_Morphism
+    `{! DecoratedTraversableFunctor W1 T}:
+    DecoratedTraversableFunctor W2 T.
+  Proof.
+    constructor.
+    - typeclasses eauto.
+    - typeclasses eauto.
+    - intros.
+      admit.
+  Admitted.
+
+
+  #[export] Instance DecoratedTraversableMonad_Monoid_Morphism
+    `{! DecoratedTraversableMonad W1 T}:
+    DecoratedTraversableMonad W2 T.
+  Proof.
+    constructor.
+    - typeclasses eauto.
+    - typeclasses eauto.
+    - typeclasses eauto.
+  Qed.
+
+End dtm_to_dtm.
