Tealeaves/Adapters/PolyToMono/Categorical/DecoratedTraversableMonad.v
@@ -1,5 +1,30 @@
 From Tealeaves Require Export
   Classes.Categorical.DecoratedTraversableMonad
   Classes.Categorical.DecoratedTraversableMonadPoly
-  Adapters.PolyToMono.Categorical.Decorated
-  Adapters.PolyToMono.Categorical.DecoratedFunctor.
+  Adapters.PolyToMono.Categorical.DecoratedFunctor
+  Adapters.PolyToMono.Categorical.DecoratedMonad
+  Adapters.PolyToMono.Categorical.TraversableMonad
+  Adapters.PolyToMono.Categorical.TraversableFunctor.
+
+Import PolyToMono.Categorical.DecoratedFunctor.ToMono1.
+Import PolyToMono.Categorical.DecoratedMonad.ToMono1.
+Import PolyToMono.Categorical.TraversableFunctor.ToMono.
+Import PolyToMono.Categorical.TraversableMonad.ToMono.
+
+#[local] Generalizable Variables T.
+
+Module ToMono.
+  Section toMono.
+
+    Context `{DecoratedTraversableMonadPoly T}.
+
+    #[export] Instance: forall B, DecoratedTraversableMonad (list B) (T B).
+    Proof.
+      intros. constructor.
+      - typeclasses eauto.
+      - typeclasses eauto.
+      - typeclasses eauto.
+    Qed.
+
+  End toMono.
+End ToMono.
