Tealeaves/Adapters/PolyToMono/Categorical/TraversableMonad.v
@@ -1,0 +1,50 @@
+From Tealeaves Require Import
+  Classes.Categorical.TraversableMonad2
+  Classes.Categorical.TraversableMonad
+  Adapters.PolyToMono.Categorical.TraversableFunctor.
+
+#[local] Generalizable Variables T G A.
+
+Import Functor2.Notations.
+Import PolyToMono.Categorical.TraversableFunctor.ToMono.
+
+(** ** Single-Argument Traversable Functor Instances *)
+(**********************************************************************)
+Module ToMono.
+
+  Section mono.
+
+    Context
+      `{TraversableMonad2 T}.
+
+    #[export] Instance TraversableMonad_Dist2_1 {B}:
+      TraversableMonad (T B).
+    Proof.
+      constructor.
+      - typeclasses eauto.
+      - typeclasses eauto.
+      - intros.
+        unfold_ops @Dist2_1.
+        reassociate -> on left.
+        rewrite dmp_map_ret.
+        reassociate <- on left.
+        rewrite (xxx_dist2_ret (T := T) B A (G := G)).
+        reflexivity.
+      - intros.
+        unfold_ops @Dist2_1.
+        reassociate -> on left.
+        rewrite dmp_map_join.
+        reassociate <- on left.
+        rewrite (xxx_dist2_join (T := T) B A (G := G)).
+        reassociate -> on left.
+        unfold_compose_in_compose.
+        setoid_rewrite fun2_map_map.
+        reassociate -> on right.
+        reassociate -> on right.
+        rewrite fun2_map2_map21.
+        reflexivity.
+    Qed.
+
+  End mono.
+
+End ToMono.
