Tealeaves/Adapters/PolyToMono/PDTM.v
@@ -1,0 +1,258 @@
+From Tealeaves Require Import
+  Categorical.DecoratedTraversableMonadPoly.
+
+From Tealeaves Require Import
+  Classes.Categorical.DecoratedFunctor
+  Classes.Categorical.RightComodule.
+
+From Tealeaves Require Import
+  Classes.Kleisli.DecoratedFunctor
+  Classes.Kleisli.DecoratedTraversableFunctor.
+
+From Tealeaves Require Import
+  Classes.Kleisli.DecoratedFunctorPoly.
+
+From Tealeaves Require Import
+  CategoricalToKleisli.DecoratedFunctor
+  CategoricalToKleisli.TraversableFunctor
+  CategoricalToKleisli.Monad
+  CategoricalToKleisli.DecoratedTraversableFunctor
+  CategoricalToKleisli.DecoratedTraversableMonad.
+
+From Tealeaves Require Import
+  CategoricalToKleisli.DecoratedFunctorPoly
+  CategoricalToKleisli.DecoratedMonadPoly
+  CategoricalToKleisli.DecoratedTraversableFunctorPoly
+  CategoricalToKleisli.DecoratedTraversableMonadPoly.
+
+From Tealeaves Require Import
+  Adapters.PolyToMono.Categorical.DecoratedFunctor
+  Adapters.PolyToMono.Categorical.TraversableFunctor
+  Adapters.PolyToMono.Categorical.TraversableMonad
+  Adapters.PolyToMono.Categorical.DecoratedMonad
+  Adapters.PolyToMono.Categorical.DecoratedTraversableMonad.
+
+From Tealeaves Require Import
+  Adapters.MonoidHom.Categorical.
+
+Module CategoricalToKleisliAll.
+  Export Adapters.PolyToMono.Categorical.DecoratedFunctor.
+  Export Adapters.PolyToMono.Categorical.DecoratedFunctor.ToMono1.
+
+  Export Adapters.PolyToMono.Categorical.TraversableFunctor.
+  Export Adapters.PolyToMono.Categorical.TraversableFunctor.ToMono.
+
+  Export Adapters.PolyToMono.Categorical.TraversableMonad.
+  Export Adapters.PolyToMono.Categorical.TraversableMonad.ToMono.
+
+  Export Adapters.PolyToMono.Categorical.DecoratedMonad.
+  Export Adapters.PolyToMono.Categorical.DecoratedMonad.ToMono1.
+
+  Export Adapters.PolyToMono.Categorical.DecoratedTraversableMonad.
+  Export Adapters.PolyToMono.Categorical.DecoratedTraversableMonad.ToMono.
+
+  Export CategoricalToKleisli.DecoratedFunctor.
+  Export CategoricalToKleisli.DecoratedFunctor.DerivedOperations.
+  Export CategoricalToKleisli.DecoratedFunctor.DerivedInstances.
+
+  Export CategoricalToKleisli.DecoratedFunctor.
+  Export CategoricalToKleisli.DecoratedFunctor.DerivedOperations.
+  Export CategoricalToKleisli.DecoratedFunctor.DerivedInstances.
+
+  Export CategoricalToKleisli.TraversableFunctor.
+  Export CategoricalToKleisli.TraversableFunctor.DerivedOperations.
+  Export CategoricalToKleisli.TraversableFunctor.DerivedInstances.
+
+  Export CategoricalToKleisli.DecoratedTraversableFunctor.
+  Export CategoricalToKleisli.DecoratedTraversableFunctor.DerivedOperations.
+  Export CategoricalToKleisli.DecoratedTraversableFunctor.DerivedInstances.
+
+  Export CategoricalToKleisli.DecoratedTraversableMonad.
+  Export CategoricalToKleisli.DecoratedTraversableMonad.DerivedOperations.
+  Export CategoricalToKleisli.DecoratedTraversableMonad.DerivedInstances.
+
+  Export CategoricalToKleisli.Monad.
+  Export CategoricalToKleisli.Monad.DerivedOperations.
+  Export CategoricalToKleisli.Monad.DerivedInstances.
+
+  Export CategoricalToKleisli.DecoratedFunctorPoly.
+  Export CategoricalToKleisli.DecoratedFunctorPoly.DerivedOperations.
+  Export CategoricalToKleisli.DecoratedFunctorPoly.DerivedInstances.
+
+  Export CategoricalToKleisli.DecoratedMonadPoly.
+  Export CategoricalToKleisli.DecoratedMonadPoly.DerivedOperations.
+  Export CategoricalToKleisli.DecoratedMonadPoly.DerivedInstances.
+
+  Export CategoricalToKleisli.DecoratedTraversableFunctorPoly.
+  Export CategoricalToKleisli.DecoratedTraversableFunctorPoly.DerivedOperations.
+  Export CategoricalToKleisli.DecoratedTraversableFunctorPoly.DerivedInstances.
+
+  Export CategoricalToKleisli.DecoratedTraversableMonadPoly.
+  Export CategoricalToKleisli.DecoratedTraversableMonadPoly.DerivedOperations.
+  Export CategoricalToKleisli.DecoratedTraversableMonadPoly.DerivedInstances.
+
+End CategoricalToKleisliAll.
+
+
+(** * Convenient Interface to categorically-defined PDTMs *)
+(********************************************************************)
+Module PDTM_specialized_ops.
+
+Section pdtm.
+
+  Context
+    {T: Type -> Type -> Type}.
+
+  Context
+    {Map2_T: Map2 T}
+    {Decorate2_T: DecoratePoly T}
+    {Dist2_T: ApplicativeDist2 T}
+    {Join_T: forall B, Join (T B)}
+    {Ret_T: forall B, Return (T B)}.
+
+  Context `{! Categorical.DecoratedTraversableMonadPoly.DecoratedTraversableMonadPoly T}.
+
+  Import CategoricalToKleisli.DecoratedFunctorPoly.DerivedOperations.
+
+  (** ** Single-argument Categorical Operations *)
+  (********************************************************************)
+  #[export] Instance vdec {B: Type}: Decorate (list B) (T B) :=
+    PolyToMono.Categorical.DecoratedFunctor.ToMono1.VDec.
+
+  #[export] Instance bdec {V: Type}: RightCoaction (fun B => T B V) Z :=
+    PolyToMono.Categorical.DecoratedFunctor.ToMono2.BDec.
+
+  #[global] Arguments vdec {B}%type_scope {V} _ :rename.
+  #[global] Arguments bdec {V}%type_scope {B} _ :rename.
+
+  #[export] Instance vdist {B: Type}: ApplicativeDist (T B) :=
+    PolyToMono.Categorical.TraversableFunctor.ToMono.Dist2_1.
+
+  #[export] Instance bdist {V: Type}: ApplicativeDist (fun B => T B V) :=
+        PolyToMono.Categorical.TraversableFunctor.ToMono.Dist2_2.
+
+  (** ** Single-argument Categorical Instances *)
+  (********************************************************************)
+  #[export] Instance DecoratedFunctor_PDTM_V: forall B,
+      @Categorical.DecoratedFunctor.DecoratedFunctor (list B) (T B) (@vmap T Map2_T B) (@vdec B) :=
+    @PolyToMono.Categorical.DecoratedFunctor.ToMono1.DecoratedFunctor_V T Map2_T Decorate2_T _.
+
+  #[export] Instance TraversableFunctor_PDTM_V: forall B,
+      @Categorical.TraversableFunctor.TraversableFunctor (T B) (@vmap T Map2_T B) (@vdist B) :=
+    @PolyToMono.Categorical.TraversableFunctor.ToMono.TraversableFunctor_Dist2_1 T Map2_T Dist2_T _.
+
+  #[export] Instance DecoratedFunctor_PDTM_B: forall V,
+      @RightComodule (fun B => T B V) Z (Map_Z) (Cojoin_Z) (Extract_Z)
+        (@bmap T Map2_T V) (@bdec V) :=
+    @PolyToMono.Categorical.DecoratedFunctor.ToMono2.DecoratedFunctor_B T Map2_T Decorate2_T _.
+
+  #[export] Instance TraversableFunctor_PDTM_B: forall V,
+      @Categorical.TraversableFunctor.TraversableFunctor (fun B => T B V) (@bmap T Map2_T V) (@bdist V) :=
+    @PolyToMono.Categorical.TraversableFunctor.ToMono.TraversableFunctor_Dist2_2 T Map2_T Dist2_T _.
+
+  (** ** Single-argument Kleisli operations *)
+  (********************************************************************)
+  #[export] Instance vtraverse {B}: Traverse (T B) :=
+    CategoricalToKleisli.TraversableFunctor.DerivedOperations.Traverse_Categorical (T B).
+
+  #[export] Instance btraverse {V}: Traverse (fun B => T B V) :=
+    CategoricalToKleisli.TraversableFunctor.DerivedOperations.Traverse_Categorical (fun B => T B V).
+
+  #[export] Instance Kleisli_TraversableFunctor_PDTM_V {B: Type}:
+      @Kleisli.TraversableFunctor.TraversableFunctor (T B) (@vtraverse B) :=
+    CategoricalToKleisli.TraversableFunctor.DerivedInstances.TraversableFunctor_Kleisli_Categorical.
+
+  #[export] Instance Kleisli_TraversableFunctor_PDTM_B {V: Type}:
+      @Kleisli.TraversableFunctor.TraversableFunctor (fun B => T B V) (@btraverse V) :=
+    CategoricalToKleisli.TraversableFunctor.DerivedInstances.TraversableFunctor_Kleisli_Categorical.
+
+  #[global] Arguments vtraverse {B}%type_scope {G Map_G Pure_G Mult_G A B} _ _.
+  #[global] Arguments btraverse {V}%type_scope {G Map_G Pure_G Mult_G A B} _ _.
+
+  #[export] Instance vmapd {B: Type}:
+    Mapd (list B) (T B) :=
+    DerivedOperations.Mapd_Categorical (Decorate_EF := @vdec B) (list B) (T B).
+
+  Definition bmapd {V B1 B2: Type}:
+    (list B1 * B1 -> B2) ->
+    T B1 V -> T B2 V :=
+    (fun f => bmap f ∘ bdec).
+
+  #[global] Arguments vmapd {B}%type_scope {V1 V2}%type_scope _ _ :rename.
+
+  #[export] Instance Compat_VMapd_Categorical_PDTM {B}:
+    Compat_Mapd_Categorical (list B) (T B).
+  Proof.
+    reflexivity.
+  Qed.
+
+  #[export] Instance Kleisli_DecoratedFunctor_PDTM_V {B: Type}:
+      @Kleisli.DecoratedFunctor.DecoratedFunctor (list B) (T B) (@vmapd B) :=
+    CategoricalToKleisli.DecoratedFunctor.DerivedInstances.DecoratedFunctor (T B).
+
+  Lemma mapdp_decompose {B1 V1 B2 V2: Type}:
+    forall (g: list B1 * B1 -> B2)
+      (f: list B1 * V1 -> V2),
+      mapdp (T := T) g f = bmapd g ∘ vmapd f.
+  Proof.
+    intros.
+    unfold_ops @Mapdp_Categorical.
+    unfold bmapd.
+    unfold vmapd.
+    unfold_ops @DerivedOperations.Mapd_Categorical.
+    unfold bmap.
+    unfold_ops @Map2_1.
+    unfold_ops @Map2_2.
+    unfold bdec.
+    unfold_ops @DecoratedFunctor.ToMono2.BDec.
+    reassociate <- on right.
+    reassociate <- on right.
+    reassociate -> near (map2 id f).
+    rewrite polydecnat.
+    reassociate <- on right.
+    rewrite fun2_map_map.
+    rewrite fun2_map_map.
+    unfold dec.
+    unfold vdec.
+    unfold DecoratedFunctor.ToMono1.VDec.
+    reassociate <- on right.
+    reassociate -> near (map2 (@extract Z Extract_Z B1) (@id (L B1 V1))).
+    rewrite polydecnat.
+    reassociate -> on right.
+    reassociate -> on right.
+    reassociate -> on right.
+    reassociate -> on right.
+    rewrite dfunp_dec_dec.
+    reassociate <- on right.
+    reassociate <- on right.
+    reassociate <- on right.
+    reassociate <- on right.
+    rewrite fun2_map_map.
+    rewrite fun2_map_map.
+    repeat rewrite fun_map_id.
+    repeat change (id ∘ ?f) with f.
+    repeat change (?f ∘ id) with f.
+    reassociate -> on right.
+    setoid_rewrite com_map_extr_cojoin.
+    repeat change (?f ∘ id) with f.
+    fequal.
+    fequal.
+    ext [l v1].
+    reflexivity.
+  Qed.
+
+  #[export] Instance vmapdt {B: Type}:
+    Mapdt (list B) (T B) :=
+    DerivedOperations.Mapdt_Categorical (Decorate_T := @vdec B) (list B) (T B).
+
+  Import CategoricalToKleisli.DecoratedTraversableFunctor.DerivedOperations.
+  Import CategoricalToKleisli.DecoratedTraversableFunctor.DerivedInstances.
+
+  #[export] Instance: forall B, DecoratedTraversableFunctor (list B) (T B).
+  Proof.
+    typeclasses eauto.
+  Qed.
+
+End pdtm.
+
+End PDTM_specialized_ops.
