Tealeaves/Backends/Adapters/LNtoNominal.v
@@ -1,0 +1,110 @@
+From Tealeaves Require Import
+  Classes.Kleisli.DecoratedFunctorPoly
+  Backends.Nominal.Common.Binding
+  Backends.Nominal.Common.Freshening
+  Backends.LN.LN.
+
+Import List.ListNotations.
+Import ContainerFunctor.Notations.
+
+(** * Converting a depth to (list unit) binding context *)
+(**********************************************************************)
+Fixpoint length_to_list_unit (length: nat): list unit :=
+  match length with
+  | 0 => nil
+  | S n => tt :: length_to_list_unit n
+  end.
+
+Lemma length_length_to_list_unit: forall n,
+    length (length_to_list_unit n) = n.
+Proof.
+  intros. induction n.
+  - reflexivity.
+  - cbn. fequal; auto.
+Qed.
+
+Lemma length_cons {A} {a:A} {l: list A}:
+  length (a :: l) = S (length l).
+Proof.
+  reflexivity.
+Qed.
+
+Lemma length_one {A} {a:A}:
+  length [a] = 1.
+Proof.
+  reflexivity.
+Qed.
+
+Lemma length_to_list_unit_plus {n m: nat}:
+  length_to_list_unit (n + m) =
+    length_to_list_unit n ++
+      length_to_list_unit m.
+Proof.
+  induction n.
+  - reflexivity.
+  - cbn. rewrite IHn.
+    reflexivity.
+Qed.
+
+Lemma length_to_list_unit_S (n: nat):
+  length_to_list_unit (S n) = tt :: length_to_list_unit n.
+Proof.
+  reflexivity.
+Qed.
+
+Lemma length_list_unit_iso (ctx: list unit):
+  ctx = length_to_list_unit (length ctx).
+Proof.
+  induction ctx.
+  - reflexivity.
+  - cbn. destruct a.
+    rewrite IHctx.
+    rewrite length_length_to_list_unit.
+    reflexivity.
+Qed.
+
+(** * Locally Nameless to Nominal *)
+(**********************************************************************)
+
+Section with_DTM.
+
+  Context
+    {T: Type -> Type -> Type}.
+
+  (* if you are going to crash, do so very loudly *)
+  Definition PANIC_INDEX_EXCEEDS_CONTEXT: nat := 1337.
+
+  (* Give a DB index (Bd N), define its new name *)
+  Definition bdToName (Γ: list name) (ctx: list unit) (n: nat): atom :=
+    if Nat.ltb n (length ctx)
+    then assignNames_loc Γ (length_to_list_unit (length ctx - (n + 1)), tt)
+    else PANIC_INDEX_EXCEEDS_CONTEXT.
+
+  Lemma bdToName_fresh: forall Γ a ctx n,
+      length ctx > n ->
+      a ∈ Γ -> bdToName Γ ctx n <> a.
+  Proof.
+    introv Hlt Hin.
+    unfold bdToName.
+    apply PeanoNat.Nat.ltb_lt in Hlt.
+    rewrite Hlt.
+    intro contra.
+    subst.
+    apply assignNames_loc_fresh in Hin.
+    assumption.
+  Qed.
+
+  Definition lnToNom_loc (Γ: list name):
+    list unit * LN -> name :=
+    fun '(depth, v) =>
+      match v with
+      | Fr x => x
+      | Bd n => bdToName Γ depth n
+      end.
+
+  Definition lnToNom `{MapdPoly T} (Γ: list name):
+    T unit LN -> T name name :=
+    mapdp (T := T) (assignNames_loc Γ) (lnToNom_loc Γ).
+
+End with_DTM.
+
