Tealeaves/Backends/Adapters/NominaltoLN.v
@@ -1,0 +1,33 @@
+From Tealeaves Require Import
+  Classes.Kleisli.DecoratedFunctorPoly
+  Backends.Nominal.Common.Binding
+  Backends.LN.LN.
+
+(** * Nominal to Locally Translation *)
+(********************************************************************)
+Section with_DTM.
+
+  Context
+    {T: Type -> Type -> Type}.
+
+  Definition binding_to_ln: Binding -> LN :=
+    fun b =>
+      match b with
+      | Bound prefix var postfix =>
+          Bd (length postfix)
+      | Unbound context var =>
+          Fr var
+      end.
+
+  Definition nomToLN_loc:
+    list name * name -> LN.
+  Proof.
+    intros [ctx x].
+    exact (binding_to_ln (get_binding ctx x)).
+  Defined.
+
+  Definition nomToLN `{MapdPoly T}:
+    T name name -> T unit LN :=
+    mapdp (T := T) (const tt) nomToLN_loc.
+
+End with_DTM.
