Tealeaves/Examples/Lambda/Intrinsic.v
@@ -1,0 +1,59 @@
+From Coq Require Import
+  Relations.Relations
+  Classes.RelationClasses.
+From Tealeaves Require Import
+  Backends.DB.
+
+
+
+
+Import DecoratedTraversableMonad.UsefulInstances.
+
+#[local] Set Implicit Arguments.
+
+Import DB.Notations.
+
+Open Scope nat_scope.
+Open Scope nat_scope.
+
+Definition incr {A}: (nat -> A) -> nat -> (nat -> A) :=
+  fun f n m => f (n + m).
+
+Inductive lam (V: nat -> Type) :=
+| tvar: V 0 -> lam V
+| abs: lam (incr V 1) -> lam V
+| app: lam V -> lam V -> lam V.
+
+Definition closed_terms := lam (Fin.t).
+
+
+Definition level_terms {n:nat} := lam (incr Fin.t n).
+
+Fixpoint binddt_lam (G: Type -> Type) `{Map G} `{Pure G} `{Mult G}
+    {v1 v2: Type} (f: nat * v1 -> G (lam v2)) (t: lam v1): G (lam v2) :=
+  match t with
+  | tvar v    => f (0, v)
+  | abs body  => pure (@abs v2) <⋆> binddt_lam (f ⦿ 1) body
+  | app t1 t2 => pure (@app v2) <⋆> binddt_lam f t1 <⋆> binddt_lam f t2
+  end.
+
+#[export] Instance Return_Lam: Return lam := tvar.
+#[export] Instance Binddt_Lam: Binddt nat lam lam := @binddt_lam.
+#[export] Instance DTM_Lam: DecoratedTraversableMonad nat lam.
+Proof.
+  derive_dtm.
+Qed.
+
+#[export] Instance DTM_Lam_Explicit: DecoratedTraversableMonad nat lam.
+Proof.
+  constructor.
+  - typeclasses eauto.
+  - intros.
+    reflexivity.
+  - constructor.
+    + intros. ext t.
+      induction t as [v | t | t1 IHt1 t2 IHt2 ].
+      * reflexivity.
+      * cbn.
+        unfold id.
+        simplify_applicative_I.
